theories/Monad.v
@@ -2,6 +2,10 @@ From LogRel.AutoSubst Require Import core unscoped Ast Extra.
 Require Import PeanoNat.
 From LogRel Require Import Utils BasicAst Notations Context LContexts NormalForms Weakening GenericTyping.
 
+Set Primitive Projections.
+Set Universe Polymorphism.
+Set Polymorphic Inductive Cumulativity.
+
 Definition Type_le_step (wl : wfLCon) (n : nat) (ne : not_in_LCon wl n) (b : bool)
   (P : forall wl', wl' ≤ε wl -> Type) : 
   forall wl', wl' ≤ε wl,,l (ne, b) -> Type :=
@@ -46,7 +50,7 @@ Definition dPred_le_down (wl wl' : wfLCon) (f: wl' ≤ε wl)
   fun wl'' f' p q => R wl'' (wfLCon_le_trans f' f) p q.
 Arguments dPred_le_down [_ _] _ [_ _] _ [_] _.
 
-Inductive Dial@{i} (wl : wfLCon) (P : forall wl', wl' ≤ε wl -> Type@{i}) : Type@{i} :=
+(*Inductive Dial@{i} (wl : wfLCon) (P : forall wl', wl' ≤ε wl -> Type@{i}) : Type@{i} :=
 | eta : P wl (wfLCon_le_id _) -> Dial wl P
 | ϝdig {n} {ne : not_in_LCon (pi1 wl) n} :
   Dial (wl ,,l (ne, true)) (Type_le_step P) ->
@@ -100,10 +104,13 @@ Fixpoint dBType2 (wl : wfLCon)
   | eta _ _ x => fun q r => S wl (wfLCon_le_id _) x q r
   | ϝdig _ _ pt pf => fun q r => let (qt, qf) := q in
                                  let (rt, rf) := r in
-                                 prod (dBType2 _ _ _ (fun wl' f p q =>
-                                                        R wl' (wfLCon_le_trans f (LCon_le_step _ (wfLCon_le_id _))) p q) pt qt)
-                                 (dBType _ _ _ (dPred_le_step R) pf qf)
-          end.
+                                 prod (dBType2 _ _ _ _
+                                         (fun wl' f p q =>
+                                            S wl' (f •ε (LCon_le_step _ (wfLCon_le_id _))) p q) pt qt rt)
+                                      (dBType2 _ _ _ _
+                                         (fun wl' f p q =>
+                                            S wl' (f •ε (LCon_le_step _ (wfLCon_le_id _))) p q) pf qf rf)
+  end.
 
 (*Fixpoint BType_dep (wl : wfLCon) (P : wfLCon -> Type)
   (Q : forall wl', P wl' -> Type)
@@ -115,4 +122,29 @@ Fixpoint dBType2 (wl : wfLCon)
   | ϝdig _ _ pt pf => fun H => prod (BType_dep _ P Q R pt (fst H))
                                  (BType_dep _ P Q R pf (snd H))
   end.
+ *)
 *)
+Inductive DTree (k : wfLCon) : Type :=
+| leaf : DTree k
+| ϝnode {n} {ne : not_in_LCon (pi1 k) n} :
+  DTree (k ,,l (ne, true)) ->
+  DTree (k ,,l (ne, false)) ->
+  DTree k.
+
+Inductive over_tree (k k' : wfLCon) :
+  DTree k -> Type :=
+| over_leaf : k' ≤ε k -> over_tree k k' (leaf k)
+| over_nodeT {n} {ne : not_in_LCon (pi1 k) n} kt kf :
+  in_LCon k' n true ->
+  over_tree (k ,,l (ne, true)) k' kt ->
+  over_tree k k' (ϝnode (ne := ne) k kt kf)
+| over_nodeF {n} {ne : not_in_LCon (pi1 k) n} kt kf :
+  in_LCon k' n false ->
+  over_tree (k ,,l (ne, false)) k' kf ->
+  over_tree k k' (ϝnode (ne := ne) k kt kf).
+
+Lemma over_tree_le k k' d : over_tree k k' d -> k' ≤ε k.
+Proof.
+  induction 1 as [ | ???????? IH | ???????? IH] ; [assumption | | ].
+  all: exact (IH •ε (LCon_le_step _ (wfLCon_le_id _))).
+Qed.
